Abstract further from predicates in constraint solver

theories/Predicates.v
@@ -28,11 +28,14 @@
 
 From Coq Require Import
   Classes.Morphisms
+  Classes.Morphisms_Prop
   Classes.RelationClasses
   Relations.Relation_Definitions.
 From Em Require Import
   Context
   Definitions
+  Environment
+  Substitution
   STLC.
 
 Set Implicit Arguments.
@@ -109,10 +112,37 @@ Module Pred.
     Proof. firstorder. Qed.
     #[export] Instance proper_pimpl : Proper (BiEntails ==> BiEntails ==> BiEntails) PImpl.
     Proof. firstorder. Qed.
-    #[export] Instance proper_pand : Proper (BiEntails ==> BiEntails ==> BiEntails) PAnd.
+    #[export] Instance proper_pand_bientails : Proper (BiEntails ==> BiEntails ==> BiEntails) PAnd.
+    Proof. firstorder. Qed.
+    #[export] Instance proper_pand_entails : Proper (Entails ==> Entails ==> Entails) PAnd.
     Proof. firstorder. Qed.
 
   End Connectives.
+
+  Definition Forall {I : TYPE} : ⊢ (I -> Pred) -> Pred :=
+    fun w A ι => forall i : I w, A i ι.
+  Definition Exists {I : TYPE} : ⊢ (I -> Pred) -> Pred :=
+    fun w A ι => exists i : I w, A i ι.
+  #[global] Arguments Forall {I w} A ι.
+  #[global] Arguments Exists {I w} A ι.
+
+  Notation "'∀' x ∶ T , Q" :=
+      (@Forall T _ (fun x => Q%P))
+        (at level 99, x binder, right associativity,
+          format "'∀'  x  ∶  T ,  Q")
+      : pred_scope.
+
+  (* Notation "'∃' x .. y , Q " := *)
+  (*     (Exists (fun x => .. (Exists (fun y => Q%P)) ..)) *)
+  (*       (at level 94, x binder, y binder, right associativity) *)
+  (*     : pred_scope. *)
+
+  Notation "'∃' x ∶ T , Q" :=
+      (@Exists T _ (fun x => Q%P))
+        (at level 99, x binder, right associativity,
+          format "'∃'  x  ∶  T ,  Q")
+      : pred_scope.
+
 
   (* #[export] Instance proper_iff_impl {w} : *)
   (*   Proper (BiEntails ==> BiEntails ==> Basics.flip Basics.impl) (@BiEntails w). *)
@@ -133,8 +163,8 @@ Module Pred.
   Proof. unfold Entails, PAnd, PImpl. intuition. Qed.
 
   Lemma split_bientails {w} (P Q : Pred w) :
-    Entails P Q -> Entails Q P -> BiEntails P Q.
-  Proof. intros PQ QP ι. split; [apply PQ|apply QP]. Qed.
+    BiEntails P Q <-> Entails P Q /\ Entails Q P.
+  Proof. unfold Entails, BiEntails. firstorder. Qed.
 
   Lemma pand_comm {w} (P Q : Pred w) : P ∧ Q ⊣⊢ Q ∧ P.
   Proof. unfold BiEntails, PAnd. intuition. Qed.
@@ -142,10 +172,36 @@ Module Pred.
   Proof. now unfold BiEntails, PAnd, PTrue. Qed.
   Lemma pand_true_r {w} (P : Pred w) : P ∧ ⊤ ⊣⊢ P.
   Proof. now unfold BiEntails, PAnd, PTrue. Qed.
+  Lemma pand_false_l {w} (P : Pred w) : PFalse ∧ P ⊣⊢ PFalse.
+  Proof. now unfold BiEntails, PAnd, PFalse. Qed.
+  Lemma pand_false_r {w} (P : Pred w) : P ∧ PFalse ⊣⊢ PFalse.
+  Proof. now unfold BiEntails, PAnd, PFalse. Qed.
   Lemma pimpl_true_l {w} (P : Pred w) : ⊤ ⇒ P ⊣⊢ P.
   Proof. unfold BiEntails, PImpl, PTrue. intuition. Qed.
   Lemma pimpl_true_r {w} (P : Pred w) : P ⇒ ⊤ ⊣⊢ ⊤.
   Proof. unfold BiEntails, PImpl, PTrue. intuition. Qed.
+  Lemma entails_true {w} (P : Pred w) : Entails P PTrue.
+  Proof. easy. Qed.
+
+  Lemma pPoseProof {w} {P Q R : Pred w} :
+    PValid Q -> Entails (P ∧ Q)%P R -> Entails P R.
+  Proof. unfold PValid, Entails, PAnd. intuition. Qed.
+
+  Lemma pGeneralize {w} {P Q R : Pred w} :
+    PValid Q -> Entails P (Q ⇒ R)%P -> Entails P R.
+  Proof. unfold PValid, Entails, PAnd. intuition. Qed.
+
+  Lemma pApply {w} {P Q R : Pred w} :
+    Entails P Q -> Entails Q R -> Entails P R.
+  Proof. apply transitivity. Qed.
+
+  Lemma pApply_r {w} {P Q R : Pred w} :
+    Entails Q R -> Entails P Q -> Entails P R.
+  Proof. intros; etransitivity; eauto. Qed.
+
+  Lemma pIntro {w} {P Q : Pred w} :
+    Entails P Q -> PValid (P ⇒ Q).
+  Proof. now unfold PValid, Entails, PImpl. Qed.
 
   Section Ext.
 
@@ -232,6 +288,159 @@ Module Pred.
       | nil       => PTrue
       | cons y ys => PAnd (instpred y) (ip ys)
       end.
+
+  Notation Expr := (Lifted expr).
+
+  Definition TPB : ⊢ Env -> Const expr -> Ty -> Expr -> Pred :=
+    fun w G e t ee ι => inst G ι |-- e ; inst t ι ~> inst ee ι.
+  #[global] Arguments TPB [w] G e t ee ι.
+  Notation "G |-- E ; T ~> EE" := (TPB G E T EE) : pred_scope.
+
+  Module Acc.
+    Import (hints) Sub.
+    Section WithAccessibilityRelation.
+      Context {R : ACC} {instR : forall w, Inst (R w) (Assignment w)}.
+
+      Definition wp {w0 w1} (r01 : R w0 w1) (Q : Pred w1) : Pred w0 :=
+        fun ι0 => exists (ι1 : Assignment w1), inst r01 ι1 = ι0 /\ Q ι1.
+      Definition wlp {w0 w1} (r01 : R w0 w1) (Q : Pred w1) : Pred w0 :=
+        fun ι0 => forall (ι1 : Assignment w1), inst r01 ι1 = ι0 -> Q ι1.
+
+      #[local] Arguments wp {_ _} _ _ _/.
+      #[local] Arguments wlp {_ _} _ _ _/.
+      #[local] Arguments PAnd {_} _ _ _/.
+      #[local] Arguments PImpl {_} _ _ _/.
+      #[local] Arguments Ext {_ _} [w] _ [_] _ _/.
+      #[local] Arguments PEq [w] _ _ _/.
+
+      #[export] Instance proper_wp_bientails {w0 w1} (r01 : R w0 w1) :
+        Proper (BiEntails ==> BiEntails) (@wp w0 w1 r01).
+      Proof.
+        intros p q pq ι. cbn. apply ex_iff_morphism.
+        intros ι1. apply and_iff_morphism. easy. apply pq.
+      Qed.
+
+      #[export] Instance proper_wp_entails {w0 w1} (r01 : R w0 w1) :
+        Proper (Entails ==> Entails) (@wp w0 w1 r01).
+      Proof.
+        intros p q pq ι. cbn. intros (ι0 & Heq & HP).
+        exists ι0. split. easy. now apply pq.
+      Qed.
+
+      #[export] Instance proper_wlp_bientails {w0 w1} (r01 : R w0 w1) :
+        Proper (BiEntails ==> BiEntails) (@wlp w0 w1 r01).
+      Proof.
+        intros p q pq ι. cbn. apply all_iff_morphism. intros ι1.
+        now apply iff_iff_iff_impl_morphism.
+      Qed.
+
+      #[export] Instance proper_wlp_entails {w0 w1} (r01 : R w0 w1) :
+        Proper (Entails ==> Entails) (@wlp w0 w1 r01).
+      Proof. intros P Q HPQ ι HP ι0 Heq. now apply HPQ, HP. Qed.
+
+      Lemma wp_refl {reflR : Refl R} {instReflR : InstRefl R}
+        {w} (Q : Pred w) : wp refl Q ⊣⊢ Q.
+      Proof.
+        split; cbn.
+        - intros (ι' & Heq & HQ). rewrite inst_refl in Heq. now subst.
+        - intros HQ. exists ι. split. now rewrite inst_refl. easy.
+      Qed.
+
+      Lemma wp_trans {transR : Trans R}
+        {w0 w1 w2} (r01 : R w0 w1) (r12 : R w1 w2) Q :
+        wp (r01 ⊙ r12) Q ⊣⊢ wp r01 (wp r12 Q).
+      Proof.
+        split; cbn.
+        - intros (ι2 & Heq & HQ). rewrite inst_trans in Heq.
+          exists (inst r12 ι2). split. easy. now exists ι2.
+        - intros (ι1 & Heq1 & ι2 & Heq2 & HQ). exists ι2.
+          split; [|easy]. rewrite inst_trans. congruence.
+      Qed.
+
+      Lemma wp_false {w0 w1} (r01 : R w0 w1) :
+        wp r01 PFalse ⊣⊢ PFalse.
+      Proof. firstorder. Qed.
+
+      Lemma and_wp_l {w0 w1} (r01 : R w0 w1) P Q :
+        wp r01 P ∧ Q ⊣⊢ wp r01 (P ∧ Ext Q r01).
+      Proof.
+        split; cbn.
+        - intros [(ι1 & <- & HP) HQ]. now exists ι1.
+        - intros (ι1 & <- & HP & HQ). split; [|easy]. now exists ι1.
+      Qed.
+
+      Lemma and_wp_r {w0 w1} (r01 : R w0 w1) P Q :
+        P ∧ wp r01 Q ⊣⊢ wp r01 (Ext P r01 ∧ Q).
+      Proof. now rewrite pand_comm, and_wp_l, pand_comm. Qed.
+
+      Lemma wp_thick {thickR : Thick R} {instThickR : InstThick R}
+        {w x} (xIn : ctx.In x w) (t : Ty (ctx.remove xIn)) Q :
+        Entails ((Ty_hole xIn ≃ thin xIn t) ∧ wlp (thick x t) Q)%P (wp (thick x t) Q).
+      Proof.
+        intros ι. cbn. intros [Heq HQ].
+        exists (env.remove _ ι xIn).
+        rewrite inst_thick.
+        rewrite Sub.subst_thin in Heq.
+        rewrite inst_persist_ty in Heq.
+        rewrite Sub.inst_thin in Heq.
+        rewrite <- Heq.
+        rewrite env.insert_remove.
+        split. easy. apply HQ.
+        rewrite inst_thick.
+        rewrite <- Heq.
+        now rewrite env.insert_remove.
+      Qed.
+
+      Lemma wlp_refl {reflR : Refl R} {instReflR : InstRefl R}
+        {w} (Q : Pred w) : wlp refl Q ⊣⊢ Q.
+      Proof.
+        split; cbn.
+        - intros HQ. apply HQ. now rewrite inst_refl.
+        - intros HQ ? <-. now rewrite inst_refl in HQ.
+      Qed.
+
+      Lemma wlp_trans {transR : Trans R}
+        {w0 w1 w2} (r01 : R w0 w1) (r12 : R w1 w2) Q :
+        wlp (r01 ⊙ r12) Q ⊣⊢ wlp r01 (wlp r12 Q).
+      Proof.
+        split; cbn.
+        - intros HQ ι1 Heq1 ι2 Heq2. apply HQ.
+          subst. now rewrite inst_trans.
+        - intros HQ ι2 Heq. rewrite inst_trans in Heq.
+          now apply (HQ (inst r12 ι2)).
+      Qed.
+
+      Lemma wlp_true {w0 w1} (r01 : R w0 w1) :
+        wlp r01 PTrue ⊣⊢ PTrue.
+      Proof. firstorder. Qed.
+
+      Lemma wlp_impl {w0 w1} (r01 : R w0 w1) P Q :
+        Entails (wlp r01 (P ⇒ Q)) (wlp r01 P ⇒ wlp r01 Q)%P.
+      Proof. intros ι0. cbn. intros HPQ HP ι1 <-. firstorder. Qed.
+
+      Lemma entails_wlp {w0 w1} (r01 : R w0 w1) P Q :
+        Entails (Ext P r01) Q -> Entails P (wlp r01 Q).
+      Proof. intros HPQ ι0 HP ι1 <-. revert HP. apply HPQ. Qed.
+
+      Lemma pvalid_wlp {w0 w1} (r01 : R w0 w1) Q :
+        PValid Q -> PValid (wlp r01 Q).
+      Proof. unfold PValid; cbn. firstorder. Qed.
+
+    End WithAccessibilityRelation.
+    (* #[global] Opaque wp. *)
+    (* #[global] Opaque wlp. *)
+  End Acc.
+
+  Lemma pno_cycle {w x} (xIn : ctx.In x w) (t : Ty w) :
+    Ty_subterm (Ty_hole xIn) t ->
+    Entails (Ty_hole xIn ≃ t)%P PFalse.
+  Proof.
+    intros Hsub ι Heq.
+    apply (inst_subterm ι) in Hsub. cbn in Hsub.
+    rewrite <- Heq in Hsub. now apply ty_no_cycle in Hsub.
+  Qed.
+
+  (* #[global] Opaque BiEntails Entails PAnd PImpl PEq. *)
 
 End Pred.
 Export Pred (Pred).
