theories/unification/CorrectnessWithAssignments.v
@@ -74,50 +74,14 @@ Module ProgramLogic.
   Import Pred.
 
   Definition WP {A} : ⊢ ◆A -> □(A -> Pred) -> Pred :=
-    fun w0 d Q ι0 =>
-      option.wp
-        (fun '(w1; (ζ01, a)) =>
-           exists (ι1 : Assignment w1),
-             inst ζ01 ι1 = ι0 /\ Q w1 ζ01 a ι1) d.
+    fun w0 d Q =>
+      match d with
+      | Some (w1; (r01, a)) => Acc.wp r01 (Q w1 r01 a)
+      | None                => PFalse
+      end.
+
   #[global] Arguments WP {A}%indexed_scope [w] _ _%P _.
   #[global] Instance params_wp : Params (@WP) 4 := {}.
-
-  Lemma wp_pure {A w0} (a : A w0) (Q : □(A -> Pred) w0) :
-    WP (η a) Q ⊣⊢ T Q a.
-  Proof.
-    unfold BiEntails, WP, η. intros ι0. rewrite option.wp_match.
-    split.
-    - intros (ι1 & e & HQ). now subst.
-    - intros HQ. exists ι0. auto.
-  Qed.
-
-  Lemma wp_bind {A B w0} (d : ◆A w0) (f : □(A -> ◆B) w0) (Q : □(B -> Pred) w0) :
-    WP (bind d f) Q ⊣⊢ WP d (fun w1 ζ1 a1 => WP (f w1 ζ1 a1) (_4 Q ζ1)).
-  Proof.
-    unfold BiEntails, WP, bind, acc. intros ι0.
-    rewrite option.wp_bind.
-    option.tactics.mixin.
-    intros (w1 & ζ01 & a).
-    rewrite option.wp_map.
-    setoid_rewrite option.wp_match.
-    destruct (f w1 ζ01 a) as [(w2 & ζ2 & b2)|]; [|firstorder].
-    split.
-    - intros (ι2 & e1 & HQ). subst. exists (inst ζ2 ι2).
-      split; [rewrite inst_trans|]; firstorder.
-    - intros (ι1 & e0 & ι2 & e1 & HQ). subst. exists ι2.
-      split; [rewrite inst_trans|]; firstorder.
-  Qed.
-
-  Lemma wp_monotonic {A w} (d : ◆A w) (R : Pred w) (P Q : □(A -> Pred) w) :
-    (forall w1 (r : w ⊒⁻ w1) (a : A w1), Entails (Ext R r) (P w1 r a ⇒ Q w1 r a)%P) ->
-    Entails R (WP d P ⇒ WP d Q)%P.
-  Proof.
-    unfold Entails, PImpl, WP, Ext; intros pq ι HR.
-    apply option.wp_monotonic.
-    intros (w1 & ζ01 & a1) (ι1 & e1 & H).
-    exists ι1; split; [assumption|].
-    revert H; apply pq. now rewrite e1.
-  Qed.
 
   #[export] Instance proper_wp_bientails {A w} :
     Proper
@@ -127,10 +91,8 @@ Module ProgramLogic.
                         (pointwise_relation _ BiEntails)) ==> BiEntails))
       (@WP A w).
   Proof.
-    intros d p q pq. apply split_bientails;
-      rewrite <- pand_true_l at 1;
-      apply pimpl_and_adjoint, wp_monotonic;
-      intros * ι _; unfold PImpl; apply pq.
+    intros d p q pq. destruct d as [(w1 & r01 & a)|]; cbn; [|easy].
+    apply Acc.proper_wp_bientails. apply pq.
   Qed.
 
   #[export] Instance proper_wp_entails {A w} :
@@ -141,54 +103,47 @@ Module ProgramLogic.
                         (pointwise_relation _ Entails)) ==> Entails))
       (@WP A w).
   Proof.
-    intros d p q pq. rewrite <- pand_true_l at 1.
-    apply pimpl_and_adjoint, wp_monotonic.
-    intros * ι _. unfold PImpl. apply pq.
+    intros d p q pq. destruct d as [(w1 & r01 & a)|]; cbn; [|easy].
+    apply Acc.proper_wp_entails. apply pq.
+  Qed.
+
+  Lemma wp_monotonic' {A w} (d : ◆A w) (R : Pred w) (P Q : □(A -> Pred) w) :
+    (forall w1 (r : w ⊒⁻ w1) (a : A w1),
+        Entails (Ext R r) (P w1 r a ⇒ Q w1 r a)%P) ->
+    Entails R (WP d P ⇒ WP d Q)%P.
+  Proof.
+    intros pq. destruct d as [(w1 & r01 & a)|]; cbn.
+    - specialize (pq w1 r01 a).
+      apply pimpl_and_adjoint.
+      rewrite Acc.and_wp_r.
+      apply Acc.proper_wp_entails.
+      apply pimpl_and_adjoint.
+      apply pq.
+    - apply pimpl_and_adjoint.
+      now rewrite pand_false_r.
+  Qed.
+
+  Lemma wp_pure {A w0} (a : A w0) (Q : □(A -> Pred) w0) :
+    WP (η a) Q ⊣⊢ T Q a.
+  Proof. unfold WP, η. now rewrite Acc.wp_refl. Qed.
+
+  Lemma wp_bind {A B w0} (d : ◆A w0) (f : □(A -> ◆B) w0) (Q : □(B -> Pred) w0) :
+    WP (bind d f) Q ⊣⊢ WP d (fun w1 ζ1 a1 => WP (f w1 ζ1 a1) (_4 Q ζ1)).
+  Proof.
+    destruct d as [(w1 & r01 & a)|]; cbn; [|reflexivity].
+    destruct (f w1 r01 a) as [(w2 & r12 & b2)|]; cbn;
+      now rewrite ?Acc.wp_trans, ?Acc.wp_false.
   Qed.
 
   Definition WLP {A} : ⊢ ◆A -> □(A -> Pred) -> Pred :=
-    fun w d Q ι0 =>
-      option.wlp
-        (fun '(w1; (ζ01, a)) =>
-           forall ι1 : Assignment w1, inst ζ01 ι1 = ι0 -> Q w1 ζ01 a ι1)
-        d.
+    fun w0 d Q =>
+      match d with
+      | Some (w1; (r01, a)) => Pred.Acc.wlp r01 (Q w1 r01 a)
+      | None                => PTrue
+      end.
   #[global] Arguments WLP {A}%indexed_scope [w] _ _%P _.
-
-  Lemma wlp_pure {A w} (a : A w) (Q : □(A -> Pred) w) :
-    WLP (η a) Q ⊣⊢ T Q a.
-  Proof.
-    unfold PIff, WLP, η, T. intros ι.
-    rewrite option.wlp_match.
-    split; intros; subst; auto.
-  Qed.
-
-  Lemma wlp_bind {A B w0} (d : ◆A w0) (f : □(A -> ◆B) w0) (Q : □(B -> Pred) w0) :
-    WLP (bind d f) Q ⊣⊢ WLP d (fun _ ζ1 a1 => WLP (f _ ζ1 a1) (_4 Q ζ1)).
-  Proof.
-    unfold BiEntails, WLP, bind, acc. intros ι0.
-    rewrite option.wlp_bind.
-    option.tactics.mixin.
-    intros (w1 & ζ01 & a).
-    rewrite option.wlp_map.
-    setoid_rewrite option.wlp_match.
-    destruct (f w1 ζ01 a) as [(w2 & ζ2 & b2)|]; [|firstorder].
-    split.
-    - intros HQ ι1 e1 ι2 e2. subst. apply HQ, inst_trans.
-    - intros HQ ι2 e2. subst. apply (HQ (inst ζ2 ι2)).
-      now rewrite inst_trans. easy.
-  Qed.
-
-  Lemma wlp_monotonic {A w} (d : ◆A w) (R : Pred w) (P Q : □(A -> Pred) w) :
-    (forall w1 (r : w ⊒⁻ w1) (a : A w1), Entails (Ext R r) (P w1 r a ⇒ Q w1 r a)%P) ->
-    Entails R (WLP d P ⇒ WLP d Q)%P.
-  Proof.
-    unfold Entails, PImpl, WLP, Ext; intros pq ι HR.
-    apply option.wlp_monotonic.
-    intros (w1 & ζ01 & a1) H ι1 e1. specialize (H ι1 e1).
-    revert H; apply pq. now rewrite e1.
-  Qed.
-
   #[global] Instance params_wlp : Params (@WLP) 4 := {}.
+
   #[export] Instance proper_wlp_bientails {A w} :
     Proper
       (pointwise_relation _
@@ -197,10 +152,8 @@ Module ProgramLogic.
                         (pointwise_relation _ BiEntails)) ==> BiEntails))
       (@WLP A w).
   Proof.
-    intros d p q pq. apply split_bientails;
-      rewrite <- pand_true_l at 1;
-      apply pimpl_and_adjoint, wlp_monotonic;
-      intros * ι _; unfold PImpl; apply pq.
+    intros d p q pq. destruct d as [(w1 & r01 & a)|]; cbn; [|easy].
+    apply Acc.proper_wlp_bientails. apply pq.
   Qed.
 
   #[export] Instance proper_wlp_entails {A w} :
@@ -211,41 +164,36 @@ Module ProgramLogic.
                         (pointwise_relation _ Entails)) ==> Entails))
       (@WLP A w).
   Proof.
-    intros d p q pq. rewrite <- pand_true_l at 1.
-    apply pimpl_and_adjoint, wlp_monotonic.
-    intros * ι _. unfold PImpl. apply pq.
+    intros d p q pq. destruct d as [(w1 & r01 & a)|]; cbn; [|easy].
+    apply Acc.proper_wlp_entails. apply pq.
+  Qed.
+
+  Lemma wlp_monotonic' {A w} (d : ◆A w) (R : Pred w) (P Q : □(A -> Pred) w) :
+    (forall w1 (r : w ⊒⁻ w1) (a : A w1),
+        Entails (Ext R r) (P w1 r a ⇒ Q w1 r a)%P) ->
+    Entails R (WLP d P ⇒ WLP d Q)%P.
+  Proof.
+    intros pq. destruct d as [(w1 & r01 & a)|]; cbn.
+    - specialize (pq w1 r01 a). rewrite <- Acc.wlp_impl.
+      now apply Acc.entails_wlp.
+    - rewrite pimpl_true_r. apply entails_true.
+  Qed.
+
+  Lemma wlp_pure {A w} (a : A w) (Q : □(A -> Pred) w) :
+    WLP (η a) Q ⊣⊢ T Q a.
+  Proof. unfold WLP, η. now rewrite Acc.wlp_refl. Qed.
+
+  Lemma wlp_bind {A B w0} (d : ◆A w0) (f : □(A -> ◆B) w0) (Q : □(B -> Pred) w0) :
+    WLP (bind d f) Q ⊣⊢ WLP d (fun w1 ζ1 a1 => WLP (f w1 ζ1 a1) (_4 Q ζ1)).
+  Proof.
+    destruct d as [(w1 & r01 & a)|]; cbn; [|reflexivity].
+    destruct (f w1 r01 a) as [(w2 & r12 & b2)|]; cbn;
+      now rewrite ?Acc.wlp_trans, ?Acc.wlp_true.
   Qed.
 
   Lemma wlp_tell1 {w x} (xIn : x ∈ w) (t : Ty (w - x)) (Q : □(Unit -> Pred) w) :
-    PValid (WLP (tell1 xIn t) Q) <->
-      PValid (Q _ (thick x t) tt).
-  Proof.
-    unfold PValid, WLP, tell1.
-    split.
-    - intros H ι. specialize (H (inst (thick (R := Tri) x t) ι)).
-      rewrite option.wlp_match in H. apply (H ι eq_refl).
-    - intros H ι. rewrite option.wlp_match. intros. apply H.
-  Qed.
-
-  Lemma pPoseProof {w} {P Q R : Pred w} :
-    PValid Q -> Entails (P ∧ Q)%P R -> Entails P R.
-  Proof. unfold PValid, Entails, PAnd. intuition. Qed.
-
-  Lemma pGeneralize {w} {P Q R : Pred w} :
-    PValid Q -> Entails P (Q ⇒ R)%P -> Entails P R.
-  Proof. unfold PValid, Entails, PAnd. intuition. Qed.
-
-  Lemma pApply {w} {P Q R : Pred w} :
-    Entails P Q -> Entails Q R -> Entails P R.
-  Proof. apply transitivity. Qed.
-
-  Lemma pApply_r {w} {P Q R : Pred w} :
-    Entails Q R -> Entails P Q -> Entails P R.
-  Proof. intros; etransitivity; eauto. Qed.
-
-  Lemma pIntro {w} {P Q : Pred w} :
-    Entails P Q -> PValid (P ⇒ Q).
-  Proof. now unfold PValid, Entails, PImpl. Qed.
+    WLP (tell1 xIn t) Q ⊣⊢ Acc.wlp (thick x t) (Q _ (thick x t) tt).
+  Proof. reflexivity. Qed.
 
 End ProgramLogic.
 
@@ -276,137 +224,137 @@ Module Correctness.
 
   Section BoxedProofs.
 
-    Import (hints) Sub.
+    Import (hints) Pred.Acc Sub.
 
     Context [w] (lmgu : ▷BoxUnifier w).
-    Context (lmgu_sound : forall x (xIn : x ∈ w),
-                BoxUnifierSound (lmgu xIn)).
 
-    Lemma flex_sound_assignment {x} (xIn : x ∈ w) (t : Ty w) :
-      ⊩ WLP (flex t xIn) (Fun _ => Ext (Ty_hole xIn ≃ t)).
-    Proof.
-      unfold flex. destruct (varview t) as [y yIn|].
-      - destruct (ctx.occurs_check_view xIn yIn).
-        + rewrite wlp_pure. unfold T. now rewrite ext_refl.
-        + rewrite wlp_tell1, <- peq_persist. cbn. unfold thickIn.
-          now rewrite ctx.occurs_check_view_refl, ctx.occurs_check_view_thin.
-      - destruct (occurs_check_sound t xIn); subst; [|constructor].
-        rewrite wlp_tell1, <- peq_persist, persist_thin_thick. cbn.
-        unfold thickIn. now rewrite ctx.occurs_check_view_refl.
-    Qed.
+    Section Soundness.
+      Context (lmgu_sound : forall x (xIn : x ∈ w),
+                  BoxUnifierSound (lmgu xIn)).
 
-    Lemma boxflex_sound_assignment {x} (xIn : x ∈ w) (t : Ty w)
-      {w1} (ζ01 : w ⊒⁻ w1) :
-      ⊩ WLP (boxflex lmgu t xIn ζ01) (Fun _ => Ext (Ext (Ty_hole xIn ≃ t) ζ01)).
-    Proof.
-      unfold boxflex, Tri.box_intro_split.
-      destruct ζ01 as [|w2 y yIn ty]; folddefs.
-      - generalize (flex_sound_assignment xIn t).
-        apply proper_pvalid_entails.
-        apply proper_wlp_entails.
-        intros w2 ζ2 _.
-        now rewrite ext_refl.
-      - generalize (lmgu_sound yIn (Ty_hole xIn)[thick y ty] t[thick y ty] ζ01). clear.
-        apply proper_pvalid_entails.
-        apply proper_wlp_entails.
-        intros w3 ζ3 _.
-        now rewrite ext_trans, peq_persist.
-    Qed.
+      Lemma flex_sound_assignment {x} (xIn : x ∈ w) (t : Ty w) :
+        ⊩ WLP (flex t xIn) (Fun _ => Ext (Ty_hole xIn ≃ t)).
+      Proof.
+        unfold flex. destruct (varview t) as [y yIn|].
+        - destruct (ctx.occurs_check_view xIn yIn).
+          + rewrite wlp_pure. unfold T. now rewrite ext_refl.
+          + rewrite wlp_tell1. apply Acc.pvalid_wlp.
+            rewrite <- peq_persist. cbn. unfold thickIn.
+            rewrite ctx.occurs_check_view_refl, ctx.occurs_check_view_thin.
+            easy.
+        - destruct (occurs_check_spec xIn t); subst; [|constructor].
+          rewrite wlp_tell1, <- peq_persist, persist_thin_thick.
+          apply Acc.pvalid_wlp. cbn. unfold thickIn.
+          rewrite ctx.occurs_check_view_refl. easy.
+      Qed.
 
-    Lemma boxmgu_sound_assignment : BoxUnifierSound (boxmgu lmgu).
-    Proof.
-      intros t1 t2. pattern (boxmgu lmgu t1 t2).
-      apply boxmgu_elim; clear t1 t2.
-      - intros. apply boxflex_sound_assignment.
-      - intros. generalize (boxflex_sound_assignment xIn t ζ01).
-        now apply proper_pvalid_entails, proper_wlp_entails.
-      - intros *. now rewrite wlp_pure.
-      - constructor.
-      - constructor.
-      - intros * IH1 IH2 *. rewrite wlp_bind.
-        specialize (IH1 _ ζ01). revert IH1.
-        apply proper_pvalid_entails, proper_wlp_entails.
-        intros w2 ζ12 _. rewrite wlp_bind.
-        apply (pGeneralize (IH2 _ (ζ01 ⊙ ζ12))), wlp_monotonic.
-        intros ? ? _. rewrite wlp_pure. unfold T, _4.
-        rewrite ?trans_refl_r, ?ext_trans, ?ext_impl.
-        apply proper_ext_entails; auto.
-        apply proper_ext_entails; auto.
-        apply proper_ext_entails; auto.
-        now rewrite peq_func.
-    Qed.
+      Lemma boxflex_sound_assignment {x} (xIn : x ∈ w) (t : Ty w)
+        {w1} (ζ01 : w ⊒⁻ w1) :
+        ⊩ WLP (boxflex lmgu t xIn ζ01) (Fun _ => Ext (Ext (Ty_hole xIn ≃ t) ζ01)).
+      Proof.
+        unfold boxflex, Tri.box_intro_split.
+        destruct ζ01 as [|w2 y yIn ty]; folddefs.
+        - generalize (flex_sound_assignment xIn t).
+          apply proper_pvalid_entails.
+          apply proper_wlp_entails.
+          intros w2 ζ2 _.
+          now rewrite ext_refl.
+        - generalize (lmgu_sound yIn (Ty_hole xIn)[thick y ty] t[thick y ty] ζ01). clear.
+          apply proper_pvalid_entails.
+          apply proper_wlp_entails.
+          intros w3 ζ3 _.
+          now rewrite ext_trans, peq_persist.
+      Qed.
 
-    Context (lmgu_complete : forall x (xIn : x ∈ w),
-                BoxUnifierComplete (lmgu xIn)).
+      Lemma boxmgu_sound_assignment : BoxUnifierSound (boxmgu lmgu).
+      Proof.
+        intros t1 t2. pattern (boxmgu lmgu t1 t2).
+        apply boxmgu_elim; clear t1 t2.
+        - intros. apply boxflex_sound_assignment.
+        - intros. generalize (boxflex_sound_assignment xIn t ζ01).
+          apply proper_pvalid_entails, proper_wlp_entails.
+          intros w2 r12 _. now rewrite peq_symmetry.
+        - intros *. now rewrite wlp_pure.
+        - constructor.
+        - constructor.
+        - intros * IH1 IH2 *. rewrite wlp_bind.
+          specialize (IH1 _ ζ01). revert IH1.
+          apply proper_pvalid_entails, proper_wlp_entails.
+          intros w2 ζ12 _. rewrite wlp_bind.
+          apply (pGeneralize (IH2 _ (ζ01 ⊙ ζ12))), wlp_monotonic'.
+          intros ? ? _. rewrite wlp_pure. unfold T, _4.
+          rewrite ?trans_refl_r, ?ext_trans, ?ext_impl.
+          apply proper_ext_entails; auto.
+          apply proper_ext_entails; auto.
+          apply proper_ext_entails; auto.
+          rewrite peq_func.
+          now apply pimpl_and_adjoint.
+      Qed.
 
-    Lemma flex_complete_assignment {x} (xIn : x ∈ w) (t : Ty w) :
-      Entails
-        (Ty_hole xIn ≃ t)%P
-        (WP (flex t xIn) (fun (w0 : World) (_ : w ⊒⁻ w0) (_ : Unit w0) => ⊤%P)).
-    Proof.
-      unfold flex. destruct (varview t) as [y yIn|].
-      - destruct (ctx.occurs_check_view xIn yIn).
-        + now rewrite wp_pure.
-        + unfold Entails, WP, PEq, tell1; cbn. intros ι Heq.
-          rewrite env.lookup_thin in Heq.
-          rewrite option.wp_match.
-          exists (env.remove _ ι xIn).
-          split; [|easy].
-          rewrite inst_thick. cbn.
-          rewrite <- Heq.
-          now rewrite env.insert_remove.
-      - unfold Entails, PEq, WP, tell1; cbn; intros ι Heq.
-        rewrite option.wp_match. destruct (occurs_check_spec xIn t); subst.
-        + exists (env.remove _ ι xIn). split; [|easy].
-          rewrite inst_thick.
-          rewrite Sub.subst_thin in Heq.
-          rewrite inst_persist_ty in Heq.
-          rewrite Sub.inst_thin in Heq. rewrite <- Heq.
-          now rewrite env.insert_remove.
-        + destruct H0; [exact (H _ _ H0)|].
-          apply (inst_subterm ι) in H0. cbn in H0. rewrite <- Heq in H0.
-          now apply ty_no_cycle in H0.
-    Qed.
+    End Soundness.
 
-    Lemma boxflex_complete_assignment {x} (xIn : x ∈ w) (t : Ty w) {w1} (ζ01 : w ⊒⁻ w1) :
-      Entails
-        (Ext (Ty_hole xIn ≃ t) ζ01)
-        (WP (boxflex lmgu t xIn ζ01) (fun (w0 : World) (_ : w1 ⊒⁻ w0) (_ : Unit w0) => ⊤%P)).
-    Proof.
-      unfold boxflex, Tri.box_intro_split.
-      destruct ζ01 as [|w2 y yIn ty]; folddefs.
-      - rewrite ext_refl. apply flex_complete_assignment.
-      - change (Tri.cons ?x ?t ?r) with (thick x t ⊙ r).
-        rewrite ext_trans, <- peq_persist.
-        now apply (lmgu_complete yIn).
-    Qed.
+    Section Completeness.
+      Context (lmgu_complete : forall x (xIn : x ∈ w),
+                  BoxUnifierComplete (lmgu xIn)).
 
-    Lemma boxmgu_complete_assignment : BoxUnifierComplete (boxmgu lmgu).
-    Proof.
-      intros t1 t2. pattern (boxmgu lmgu t1 t2).
-      apply boxmgu_elim; clear t1 t2.
-      - intros. apply boxflex_complete_assignment.
-      - intros. rewrite peq_symmetry. apply boxflex_complete_assignment.
-      - intros *. now rewrite wp_pure.
-      - cbn; discriminate.
-      - cbn; discriminate.
-      - intros * IH1 IH2 *.
-        rewrite wp_bind, peq_func.
-        rewrite <- ext_and.
-        apply pimpl_and_adjoint.
-        apply (pApply (IH1 w1 ζ01)). clear IH1.
-        apply pimpl_and_adjoint.
-        rewrite pand_comm.
-        apply pimpl_and_adjoint.
-        apply wp_monotonic. intros.
-        rewrite pimpl_true_l.
-        rewrite wp_bind.
-        rewrite <- ext_trans.
-        apply (pApply (IH2 _ _)).
-        apply proper_wp_entails. intros ? ? _.
-        rewrite wp_pure. unfold _4, T.
-        reflexivity.
-    Qed.
+      Lemma flex_complete_assignment {x} (xIn : x ∈ w) (t : Ty w) :
+        Entails
+          (Ty_hole xIn ≃ t)%P
+          (WP (flex t xIn) (fun (w0 : World) (_ : w ⊒⁻ w0) (_ : Unit w0) => ⊤%P)).
+      Proof.
+        unfold flex. destruct (varview t) as [y yIn|].
+        - destruct (ctx.occurs_check_view xIn yIn).
+          + rewrite wp_pure. unfold T. apply entails_true.
+          + unfold WP, tell1. rewrite <- Acc.wp_thick.
+            now rewrite Acc.wlp_true, pand_true_r.
+        - destruct (occurs_check_spec xIn t); subst; cbn.
+          + unfold WP, tell1. rewrite <- Acc.wp_thick.
+            now rewrite Acc.wlp_true, pand_true_r.
+          + destruct H0; [destruct (H _ _ H0)|].
+            now apply pno_cycle in H0.
+      Qed.
+
+      Lemma boxflex_complete_assignment {x} (xIn : x ∈ w) (t : Ty w) {w1} (ζ01 : w ⊒⁻ w1) :
+        Entails
+          (Ext (Ty_hole xIn ≃ t) ζ01)
+          (WP (boxflex lmgu t xIn ζ01) (fun (w0 : World) (_ : w1 ⊒⁻ w0) (_ : Unit w0) => ⊤%P)).
+      Proof.
+        unfold boxflex, Tri.box_intro_split.
+        destruct ζ01 as [|w2 y yIn ty]; folddefs.
+        - rewrite ext_refl. apply flex_complete_assignment.
+        - change (Tri.cons ?x ?t ?r) with (thick x t ⊙ r).
+          rewrite ext_trans, <- peq_persist.
+          now apply (lmgu_complete yIn).
+      Qed.
+
+      Lemma boxmgu_complete_assignment : BoxUnifierComplete (boxmgu lmgu).
+      Proof.
+        intros t1 t2. pattern (boxmgu lmgu t1 t2).
+        apply boxmgu_elim; clear t1 t2.
+        - intros. apply boxflex_complete_assignment.
+        - intros. rewrite peq_symmetry. apply boxflex_complete_assignment.
+        - intros *. rewrite wp_pure. apply entails_true.
+        - admit. (* cbn; discriminate. *)
+        - admit. (* cbn; discriminate. *)
+        - intros * IH1 IH2 *.
+          rewrite wp_bind, peq_func.
+          rewrite <- ext_and.
+          apply pimpl_and_adjoint.
+          apply (pApply (IH1 w1 ζ01)). clear IH1.
+          apply pimpl_and_adjoint.
+          rewrite pand_comm.
+          apply pimpl_and_adjoint.
+          apply wp_monotonic'. intros.
+          rewrite pimpl_true_l.
+          rewrite wp_bind.
+          rewrite <- ext_trans.
+          apply (pApply (IH2 _ _)).
+          apply proper_wp_entails. intros ? ? _.
+          rewrite wp_pure. unfold _4, T.
+          reflexivity.
+      Admitted.
+
+    End Completeness.
 
   End BoxedProofs.
 
@@ -465,11 +413,11 @@ Module Correctness.
   Lemma boxsolvelist_sound {w} : BoxSolveListSound (boxsolvelist (w := w)).
   Proof.
     intros C. induction C as [|[t1 t2]]; cbn; intros.
-    - rewrite wlp_pure. unfold T. now rewrite ext_refl.
+    - rewrite Acc.wlp_refl. easy.
     - rewrite wlp_bind. generalize (bmgu_sound t1 t2 ζ01).
       apply proper_pvalid_entails, proper_wlp_entails.
       intros w2 r2 _. apply (pGeneralize (IHC _ (ζ01 ⊙⁻ r2))).
-      apply wlp_monotonic. unfold _4. intros w3 r3 _.
+      apply wlp_monotonic'. unfold _4. intros w3 r3 _.
       rewrite ?trans_refl_r, ?ext_trans, ?ext_impl.
       apply proper_ext_entails; auto.
       apply proper_ext_entails; auto.
@@ -488,14 +436,14 @@ Module Correctness.
   Lemma boxsolvelist_complete {w} : BoxSolveListComplete (boxsolvelist (w := w)).
   Proof.
     intros C. induction C as [|[t1 t2]]; cbn; intros.
-    - rewrite wp_pure. unfold T. easy.
+    - rewrite Acc.wp_refl. easy.
     - rewrite wp_bind. rewrite <- ext_and.
       apply pimpl_and_adjoint.
       apply (pApply (@bmgu_complete _ t1 t2 _ ζ01)).
       apply pimpl_and_adjoint.
       rewrite pand_comm.
       apply pimpl_and_adjoint.
-      apply wp_monotonic. intros.
+      apply wp_monotonic'. intros.
       rewrite pimpl_true_l, <- ext_trans.
       apply IHC.
   Qed.
@@ -509,79 +457,77 @@ Module Correctness.
 
   Definition wp_prenex {A} : ⊢ ?◇⁺(List (Ty * Ty) * A) -> □⁺(A -> Pred) -> Pred :=
     fun w o Q =>
-      fun ι =>
-      option.wp (fun '(w'; (r, (C, a))) =>
-          exists ι', inst r ι' = ι /\ instpred C ι' /\ Q w' r a ι') o.
+      match o with
+      | Some (w'; (r, (C, a))) => Acc.wp r (instpred C ∧ Q _ r a)
+      | None => PFalse
+      end.
 
   Lemma prenex_correct {A w} (m : FreeM A w) (Q : □⁺(A -> Pred) w) :
-    forall ι,
-      wp_prenex (prenex m) Q ι <-> STLC.WP m Q ι.
+    wp_prenex (prenex m) Q ⊣⊢ STLC.WP m Q.
   Proof.
     unfold wp_prenex.
-    induction m; intros ι; cbn.
-    - rewrite option.wp_match. unfold T. firstorder. now subst.
-    - rewrite option.wp_match. reflexivity.
-    - rewrite <- IHm. clear IHm.
-      rewrite option.wp_bind. do 2 rewrite option.wp_match.
-      destruct (prenex m) as [(w' & r & C & a)|]; [|easy].
-      rewrite option.wp_match. cbn. unfold PAnd, PEq.
-      firstorder; subst.
-      + now rewrite <- ?inst_persist_ty.
-      + exists x. now rewrite ?inst_persist_ty.
-    - setoid_rewrite <- IHm. clear IHm.
-      rewrite option.wp_bind. repeat setoid_rewrite option.wp_match.
-      destruct (prenex m) as [(w' & r & C & a)|]; [|firstorder].
-      rewrite option.wp_match. cbn. unfold PAnd, PEq, _4.
-      split.
-      + intros (ι' & Heq & HC & HQ). subst. remember (inst r ι') as ι.
-        destruct (Environment.env.view ι).
-        exists v. exists ι'. rewrite Heqι. auto.
-      + intros (t & ι' & Heq & HC & HQ).
-        exists ι'. rewrite Heq. cbn. auto.
+    induction m; cbn.
+    - rewrite Acc.wp_refl. rewrite pand_true_l. reflexivity.
+    - reflexivity.
+    - destruct (prenex m) as [(w' & r & C & a)|]; cbn.
+      + change (Acc.wp r (((t[r] ≃ t0[r]) ∧ instpred C) ∧ Q w' r a)
+          ⊣⊢ PEq t t0 ∧ STLC.WP m Q).
+        rewrite <- IHm.
+        rewrite Acc.and_wp_r.
+        apply Acc.proper_wp_bientails.
+        rewrite <- peq_persist.
+        unfold BiEntails, PAnd.
+        intros ι; cbn; intuition.
+      + change (PFalse ⊣⊢ (PEq t t0 ∧ STLC.WP m Q)).
+        rewrite <- IHm. now rewrite pand_false_r.
+    - unfold BiEntails, PAnd, PEq, _4, Acc.wp in *.
+      intros ι. destruct (prenex m) as [(w' & r & C & a)|]; cbn.
+      + split.
+        * intros (ι' & Heq & HC & HQ). subst. cbn.
+          remember (inst r ι') as ι. destruct (env.view ι).
+          exists v. apply IHm. exists ι'. rewrite Heqι.
+          split. easy. split; auto.
+        * intros (t & Hwp). apply IHm in Hwp.
+          destruct Hwp as (ι' & Heq & HC & HQ).
+          exists ι'. cbn. rewrite Heq. cbn. auto.
+      + split; [easy|]. intros (t & Hwp). now apply IHm in Hwp.
   Qed.
 
-  Definition wp_optiondiamond {A} : ⊢ ?◇⁺ A -> □⁺(A -> Pred) -> Pred.
-  Proof.
-    intros w m Q ι.
-    refine (option.wp _ m).
-    intros (w1 & r1 & a1).
-    refine (exists ι1, inst r1 ι1 = ι /\ Q _ r1 a1 ι1).
-  Defined.
+  Definition wp_optiondiamond {A} : ⊢ ?◇⁺ A -> □⁺(A -> Pred) -> Pred :=
+    fun w m Q =>
+      match m with
+      | Some (w1; (r01, a)) => Acc.wp r01 (Q w1 r01 a)
+      | None => PFalse
+      end.
 
   Lemma solvefree_equiv {A} {pA : Persistent Tri.Tri A}
     (m : FreeM A ctx.nil) (Q : □⁺(A -> Pred) [ctx]) :
     wp_optiondiamond (solvefree m) Q ⊣⊢ STLC.WP m Q.
   Proof.
-    intros ι. unfold wp_optiondiamond, solvefree.
-    rewrite option.wp_bind, <- prenex_correct.
-    unfold wp_prenex. apply option.wp_proper.
-    intros (w1 & r1 & C & a).
-    rewrite option.wp_bind.
+    rewrite <- prenex_correct. unfold solvefree.
+    unfold wp_prenex, wp_optiondiamond.
+    destruct (prenex m) as [(w1 & r1 & C & a)|]; cbn; [|easy].
     pose proof (solvelist_complete C) as Hcompl.
     pose proof (solvelist_sound C) as Hsound.
-    rewrite option.wp_match.
-    destruct solvelist as [(w2 & r2 & [])|].
-    - rewrite option.wp_match. split.
-      + intros (ι2 & Heq & HQ); subst.
-        exists (inst r2 ι2). specialize (Hsound (inst r2 ι2)).
-        unfold WLP, Ext in Hsound. rewrite option.wlp_match in Hsound.
-        specialize (Hsound ι2 eq_refl). repeat split.
+    destruct solvelist as [(w2 & r2 & [])|]; cbn in *.
+    - apply split_bientails. split.
+      + intros ι0 (ι2 & Heq & HQ); subst. exists (inst r2 ι2).
+        specialize (Hsound (inst r2 ι2) ι2 eq_refl). hnf in Hsound.
+        unfold PAnd. repeat split.
         * destruct (env.view (inst r1 (inst r2 ι2))).
           destruct (env.view (inst alloc.nil_l ι2)).
           reflexivity.
         * assumption.
         * clear - HQ. admit.
-      + intros (ι1 & Heq1 & HC & HQ).
-        specialize (Hcompl ι1 HC). unfold WP in Hcompl.
-        rewrite option.wp_match in Hcompl. destruct Hcompl as (ι2 & Heq2 & _).
+      + intros ι0 (ι1 & Heq1 & HC & HQ).
+        specialize (Hcompl ι1 HC). destruct Hcompl as (ι2 & Heq2 & _).
         exists ι2. split. subst.
         * destruct (env.view (inst r1 (inst r2 ι2))).
           destruct (env.view (inst alloc.nil_l ι2)).
           reflexivity.
         * clear - HQ. admit.
-    - split; [easy|]. intros (ι1 & Heq1 & HC & HQ).
-      specialize (Hcompl ι1 HC). unfold WP in Hcompl.
-      now rewrite option.wp_match in Hcompl.
+    - apply split_bientails. split. firstorder.
+      intros ι (ι1 & Heq & HC & HQ). apply (Hcompl ι1 HC).
   Admitted.
 
 End Correctness.
@@ -598,8 +544,8 @@ Module Generalized.
     (RQ : RProper (RBox (RImpl RUnit RPred)) Q) :
     WLP (tell1 xIn t) Q ⊣⊢ (t[Sub.thin xIn] ≃ Ty_hole xIn ⇒ T Q tt).
   Proof.
-    unfold BiEntails, WLP, PEq, PImpl, tell1, T. intros ι.
-    rewrite option.wlp_match. cbn. split.
+    rewrite wlp_tell1. unfold BiEntails, Acc.wlp, PEq, PImpl, T.
+    intros ι. cbn. split.
     - intros HQ Heq.
       rewrite inst_persist_ty, Sub.inst_thin in Heq.
       specialize (HQ (env.remove _ ι xIn)).
@@ -634,19 +580,19 @@ Module Generalized.
       + now rewrite wlp_pure, peq_refl, pimpl_true_l.
       + rewrite wlp_tell'; auto. cbn.
         now rewrite Sub.lk_thin.
-    - unfold PValid, WLP, PEq, PImpl. intros ι. rewrite option.wlp_match.
+    - unfold PValid, WLP, PEq, PImpl. intros ι.
       destruct (occurs_check_spec xIn t); cbn; subst.
       + split.
         * intros HQ Heq. specialize (HQ (env.remove _ ι xIn)).
           rewrite Sub.subst_thin, inst_persist_ty, Sub.inst_thin in Heq.
-          rewrite Heq in HQ. rewrite env.insert_remove in HQ.
+          rewrite inst_thick, Heq in HQ. rewrite env.insert_remove in HQ.
           specialize (HQ eq_refl). revert HQ. unfold T.
           specialize (RQ _ _ refl (thick x a) (thick x a) eq_refl tt tt I).
           specialize (RQ (env.remove x ι xIn)).
           rewrite inst_thick, Heq, env.insert_remove in RQ.
           apply RQ.
         * intros Heq ι1 <-.
-          rewrite Sub.subst_thin, inst_persist_ty, Sub.inst_thin in Heq.
+          rewrite inst_thick, Sub.subst_thin, inst_persist_ty, Sub.inst_thin in Heq.
           rewrite env.remove_insert, env.lookup_insert in Heq.
           specialize (Heq eq_refl). revert Heq. unfold T.
           specialize (RQ _ _ refl (thick x a) (thick x a) eq_refl tt tt I).
@@ -654,7 +600,7 @@ Module Generalized.
           apply RQ.
       + destruct H0.
         * destruct (H _ _ H0).
-        * split; auto. intros _ Heq. exfalso.
+        * split; [|easy]. intros _ Heq. exfalso.
           apply (inst_subterm ι) in H0. rewrite Heq in H0.
           now apply ty_no_cycle in H0.
   Qed.
